union find with rank spec is done.

sample_mark/verif_unionfind_rank.v
@@ -29,6 +29,11 @@ Notation Graph := (@Graph pSGG_VST nat unit unit).
 Notation uf_under_bound g := (uf_under_bound id g).
 Existing Instances maGraph finGraph liGraph RGF.
 
+Definition vlabel_in_bound (g: Graph) := forall x, vvalid g x -> Z.of_nat (vlabel g x) <= Int.max_signed.
+
+Lemma rank_unchanged_in_bound: forall (g g': Graph), uf_equiv g g' -> rank_unchanged g g' -> vlabel_in_bound g -> vlabel_in_bound g'.
+Proof. unfold uf_equiv, rank_unchanged, vlabel_in_bound. intros. destruct H as [? _]. pose proof H2. rewrite <- H in H2. rewrite <- H0; auto. Qed.
+
 Definition mallocN_spec :=
  DECLARE _mallocN
   WITH sh: wshare, n:Z
@@ -52,7 +57,7 @@ Definition find_spec :=
           SEP   (whole_graph sh g)
   POST [ tptr (Tstruct _Node noattr) ]
         EX g': Graph, EX rt : pointer_val,
-        PROP (uf_equiv g g' /\ uf_root g' x rt /\ uf_under_bound g')
+        PROP (uf_equiv g g' /\ uf_root g' x rt /\ uf_under_bound g' /\ rank_unchanged g g')
         LOCAL (temp ret_temp (pointer_val_val rt))
         SEP (whole_graph sh g').
 
@@ -60,12 +65,12 @@ Definition unionS_spec :=
  DECLARE _unionS
   WITH sh: wshare, g: Graph, x: pointer_val, y: pointer_val
   PRE [ _x OF (tptr (Tstruct _Node noattr)), _y OF (tptr (Tstruct _Node noattr))]
-          PROP  (vvalid g x /\ vvalid g y)
+          PROP  (vvalid g x /\ vvalid g y /\ uf_under_bound g /\ vlabel_in_bound g)
           LOCAL (temp _x (pointer_val_val x); temp _y (pointer_val_val y))
           SEP   (whole_graph sh g)
   POST [ Tvoid ]
         EX g': Graph,
-        PROP (uf_union g x y g')
+        PROP (uf_union g x y g' /\ uf_under_bound g')
         LOCAL()
         SEP (whole_graph sh g').
 
@@ -97,7 +102,7 @@ Proof.
     forward. forward. forward.
     change (@field_at CompSpecs sh node_type [] (Vint (Int.repr 0), pointer_val_val x)) with (@data_at CompSpecs sh node_type (Vint (Int.repr 0), pointer_val_val x)).
     apply (exp_right (make_set_Graph O tt tt x g x_not_null H0)). entailer. apply (exp_right x). entailer !.
-    + split; [|split]; simpl; [right | apply is_partial_make_set_pregraph | apply uf_under_bound_make_set_graph]; auto. 
+    + split; [|split]; simpl; [right | apply is_partial_make_set_pregraph | apply uf_under_bound_make_set_graph]; auto.
     + assert (Coqlib.Prop_join (vvalid g) (eq x) (vvalid (make_set_Graph 0%nat tt tt x g x_not_null H0))). {
         simpl; hnf; split; intros; [unfold graph_gen.addValidFunc | subst a]; intuition.
       } assert (vgamma (make_set_Graph O tt tt x g x_not_null H0) x = (O, x)). {
@@ -162,7 +167,7 @@ Proof.
   (* if (p != x) { *)
   forward_if_tac
     (EX g': Graph, EX rt : pointer_val,
-     PROP (uf_equiv g g' /\ uf_root g' x rt /\ uf_under_bound g')
+     PROP (uf_equiv g g' /\ uf_root g' x rt /\ uf_under_bound g' /\ rank_unchanged g g')
      LOCAL (temp _p (pointer_val_val rt); temp _x (pointer_val_val x))
      SEP (whole_graph sh g'));
     [apply ADMIT | | gather_current_goal_with_evar ..].
@@ -173,10 +178,10 @@ Proof.
   assert (weak_valid g' root) by (right; destruct H4; apply reachable_foot_valid in H4; auto).
   assert (vvalid g' x) by (destruct H3 as [? _]; rewrite <- H3; apply H).
   assert (~ reachable g' root x) by (apply (uf_equiv_not_reachable g g' x r pa root); auto).
-  assert (vertices_at sh (vvalid (Graph_gen_redirect_parent g' x root H7 H8 H9)) (Graph_gen_redirect_parent g' x root H7 H8 H9) =
-          vertices_at sh (vvalid g') (Graph_gen_redirect_parent g' x root H7 H8 H9)). {
+  assert (vertices_at sh (vvalid (Graph_gen_redirect_parent g' x root H8 H9 H10)) (Graph_gen_redirect_parent g' x root H8 H9 H10) =
+          vertices_at sh (vvalid g') (Graph_gen_redirect_parent g' x root H8 H9 H10)). {
     apply vertices_at_Same_set. unfold Ensembles.Same_set, Ensembles.Included, Ensembles.In. simpl. intuition. }
-  remember (vgamma g' x) as rpa eqn:?H. destruct rpa as [r' pa']. symmetry in H11.
+  remember (vgamma g' x) as rpa eqn:?H. destruct rpa as [r' pa']. symmetry in H12.
   localize
    (PROP  ()
     LOCAL (temp _p (pointer_val_val root); temp _x (pointer_val_val x))
@@ -187,25 +192,26 @@ Proof.
       repeat apply eexists_add_stats_cons; constructor
     | store_tac
     | abbreviate_semax_ram].
-    assert (force_val (sem_cast_neutral (pointer_val_val root)) = pointer_val_val root) by (destruct root; simpl; auto). rewrite H12. clear H12.
+    assert (force_val (sem_cast_neutral (pointer_val_val root)) = pointer_val_val root) by (destruct root; simpl; auto). rewrite H13. clear H13.
     change (@field_at CompSpecs sh node_type [] (Vint (Int.repr (Z.of_nat r')), pointer_val_val root) (pointer_val_val x)) with
         (@data_at CompSpecs sh node_type (Vint (Int.repr (Z.of_nat r')), pointer_val_val root) (pointer_val_val x)).
   unlocalize
    (PROP ()
     LOCAL (temp _p (pointer_val_val root); temp _x (pointer_val_val x))
-    SEP (whole_graph sh (Graph_gen_redirect_parent g' x root H7 H8 H9))).
+    SEP (whole_graph sh (Graph_gen_redirect_parent g' x root H8 H9 H10))).
   Grab Existential Variables.
   Focus 3. { Intros g' rt. forward. apply (exp_right g'). entailer !. apply (exp_right rt). entailer !. } Unfocus.
   Focus 3. {
-    forward. apply (exp_right g). apply (exp_right x). entailer ! . apply false_Cne_eq in H2. subst pa. split; [|split]; auto.
+    forward. apply (exp_right g). apply (exp_right x). entailer ! . apply false_Cne_eq in H2. subst pa. split; [|split; [split |]]; auto.
     - apply (uf_equiv_refl _  (liGraph g)).
     - apply uf_root_vgamma with (n := r); auto.
+    - repeat intro; auto.
   } Unfocus.
   Focus 2. {
-    simplify_ramif. rewrite H10. apply (@graph_gen_redirect_parent_ramify _ (sSGG_VST sh)); auto. destruct H4.
+    simplify_ramif. rewrite H11. apply (@graph_gen_redirect_parent_ramify _ (sSGG_VST sh)); auto. destruct H4.
     apply reachable_foot_valid in H4. intro. subst root. apply (valid_not_null g' null H4). simpl. auto.
   } Unfocus.
-  rewrite H10. unfold semax_ram. forward. apply (exp_right (Graph_gen_redirect_parent g' x root H7 H8 H9)). apply (exp_right root). rewrite H10. entailer !.
+  rewrite H11. unfold semax_ram. forward. apply (exp_right (Graph_gen_redirect_parent g' x root H8 H9 H10)). apply (exp_right root). rewrite H11. entailer !.
   assert (uf_root g' x root). {
     rewrite <- (uf_equiv_root_the_same g); auto. apply (uf_root_edge _ (liGraph g) _ pa); [| apply vgamma_not_dst with r | rewrite (uf_equiv_root_the_same g g')]; auto.
   } split; [|split].
@@ -237,25 +243,24 @@ Qed.
 Lemma body_unionS: semax_body Vprog Gprog f_unionS unionS_spec.
 Proof.
   start_function.
-  destruct H.
-  forward_call (sh, g, x). Intros vret. destruct vret as [g1 x_root]. simpl fst in *. simpl snd in *.
-  assert (vvalid g1 y) by (destruct H1 as [? _]; rewrite <- H1; apply H0).
-  forward_call (sh, g1, y). Intros vret. destruct vret as [g2 y_root]. simpl fst in *. simpl snd in *.
+  destruct H as [? [? [? ?]]]. forward_call (sh, g, x). Intros vret. destruct vret as [g1 x_root]. simpl fst in *. simpl snd in *. apply rank_unchanged_in_bound in H6; auto.
+  assert (vvalid g1 y) by (destruct H3 as [? _]; rewrite <- H3; apply H0).
+  forward_call (sh, g1, y). Intros vret. destruct vret as [g2 y_root]. simpl fst in *. simpl snd in *. apply rank_unchanged_in_bound in H11; auto.
   forward_if_tac
     (PROP (x_root <> y_root)
      LOCAL (temp _yRoot (pointer_val_val y_root); temp _xRoot (pointer_val_val x_root);
      temp _x (pointer_val_val x); temp _y (pointer_val_val y))
      SEP (vertices_at sh (vvalid g2) g2)). 1: apply ADMIT.
-  Focus 1. { forward. apply (exp_right g2). entailer !; auto. apply true_Ceq_eq in H6. subst y_root. apply (the_same_root_union g g1 g2 x y x_root); auto. } Unfocus.
-  Focus 1. { forward. apply false_Ceq_neq in H6. entailer. } Unfocus.
+  Focus 1. { forward. apply (exp_right g2). entailer !; auto. apply true_Ceq_eq in H12. subst y_root. apply (the_same_root_union g g1 g2 x y x_root); auto. } Unfocus.
+  Focus 1. { forward. apply false_Ceq_neq in H12. entailer. } Unfocus.
 
   (* xRank = xRoot -> rank; *)
-  Intros. remember (vgamma g2 x_root) as rpa eqn:?H. destruct rpa as [rankXRoot paXRoot]. symmetry in H7.
+  Intros. remember (vgamma g2 x_root) as rpa eqn:?H. destruct rpa as [rankXRoot paXRoot]. symmetry in H13.
   localize
     (PROP  ()
      LOCAL (temp _xRoot (pointer_val_val x_root))
      SEP  (data_at sh node_type (vgamma2cdata (vgamma g2 x_root)) (pointer_val_val x_root))).
-  rewrite H7. simpl vgamma2cdata. apply -> ram_seq_assoc.
+  rewrite H13. simpl vgamma2cdata. apply -> ram_seq_assoc.
   eapply semax_ram_seq;
   [subst RamFrame RamFrame0; unfold abbreviate;
    repeat apply eexists_add_stats_cons; constructor
@@ -268,17 +273,17 @@ Proof.
      SEP  (whole_graph sh g2)).
   Grab Existential Variables.
   Focus 2. {
-    simplify_ramif. rewrite H7. simpl. apply (@vertices_at_ramif_1_stable _ _ _ _ SGBA_VST _ _ (SGA_VST sh) g2 (vvalid g2) x_root (rankXRoot, paXRoot)); auto.
-    destruct H4 as [? _]. rewrite <- H4. destruct H2. apply reachable_foot_valid in H2. apply H2.
+    simplify_ramif. rewrite H13. simpl. apply (@vertices_at_ramif_1_stable _ _ _ _ SGBA_VST _ _ (SGA_VST sh) g2 (vvalid g2) x_root (rankXRoot, paXRoot)); auto.
+    destruct H8 as [? _]. rewrite <- H8. destruct H4. apply reachable_foot_valid in H4. apply H4.
   } Unfocus.
 
   (* yRank = yRoot -> rank; *)
-  remember (vgamma g2 y_root) as rpa eqn:?H. destruct rpa as [rankYRoot paYRoot]. symmetry in H8.
+  remember (vgamma g2 y_root) as rpa eqn:?H. destruct rpa as [rankYRoot paYRoot]. symmetry in H14.
   localize
     (PROP  ()
      LOCAL (temp _yRoot (pointer_val_val y_root))
      SEP  (data_at sh node_type (vgamma2cdata (vgamma g2 y_root)) (pointer_val_val y_root))).
-  rewrite H8. simpl vgamma2cdata. apply -> ram_seq_assoc.
+  rewrite H14. simpl vgamma2cdata. apply -> ram_seq_assoc.
   eapply semax_ram_seq;
   [subst RamFrame RamFrame0; unfold abbreviate;
    repeat apply eexists_add_stats_cons; constructor
@@ -291,25 +296,33 @@ Proof.
      SEP  (whole_graph sh g2)).
   Grab Existential Variables.
   Focus 2. {
-    simplify_ramif. rewrite H8. simpl. apply (@vertices_at_ramif_1_stable _ _ _ _ SGBA_VST _ _ (SGA_VST sh) g2 (vvalid g2) y_root (rankYRoot, paYRoot)); auto.
-    destruct H5. apply reachable_foot_valid in H5. apply H5.
+    simplify_ramif. rewrite H14. simpl. apply (@vertices_at_ramif_1_stable _ _ _ _ SGBA_VST _ _ (SGA_VST sh) g2 (vvalid g2) y_root (rankYRoot, paYRoot)); auto.
+    destruct H9. apply reachable_foot_valid in H9. apply H9.
   } Unfocus.
-
+  assert (vvalid g2 x_root) by (destruct H8 as [? _]; rewrite <- H8; destruct H4; apply reachable_foot_valid in H4; apply H4). clear H1 H2 H5 H6.
+  assert (Int.signed (Int.repr (Z.of_nat rankXRoot)) = Z.of_nat (vlabel g2 x_root)). {
+    simpl vgamma in H13. inversion H13. apply Int.signed_repr. split.
+    - pose proof Int.min_signed_neg. pose proof (Zle_0_nat rankXRoot). intuition.
+    - specialize (H11 x_root H15). auto.
+  } assert (Int.signed (Int.repr (Z.of_nat rankYRoot)) = Z.of_nat (vlabel g2 y_root)). {
+    simpl vgamma in H14. inversion H14. apply Int.signed_repr. split.
+    - pose proof Int.min_signed_neg. pose proof (Zle_0_nat rankYRoot). intuition.
+    - destruct H9 as [? _]. apply reachable_foot_valid in H2. specialize (H11 y_root H2). auto.
+  } clear H11.
   unfold semax_ram.
   forward_if_tac
     (EX g': Graph,
-     PROP (uf_union g x y g')
+     PROP (uf_union g x y g' /\ uf_under_bound g')
           LOCAL (temp _xRank (Vint (Int.repr (Z.of_nat rankXRoot))); temp _yRank (Vint (Int.repr (Z.of_nat rankYRoot)));
                  temp _xRoot (pointer_val_val x_root); temp _yRoot (pointer_val_val y_root);
                  temp _x (pointer_val_val x); temp _y (pointer_val_val y))
      SEP (whole_graph sh g')).
   Focus 3. { Intros g'. forward. apply (exp_right g'). entailer. } Unfocus.
   Focus 2. { gather_current_goal_with_evar. } Unfocus.
-  assert (weak_valid g2 y_root) by (right; destruct H5; apply reachable_foot_valid in H5; apply H5).
-  assert (vvalid g2 x_root) by (destruct H4 as [? _]; rewrite <- H4; destruct H2; apply reachable_foot_valid in H2; apply H2).
-  assert (~ reachable g2 y_root x_root) by (intro; destruct H5; specialize (H13 _ H12); auto).
-  assert (vertices_at sh (vvalid (Graph_gen_redirect_parent g2 x_root y_root H10 H11 H12)) (Graph_gen_redirect_parent g2 x_root y_root H10 H11 H12) =
-          vertices_at sh (vvalid g2) (Graph_gen_redirect_parent g2 x_root y_root H10 H11 H12)). {
+  assert (weak_valid g2 y_root) by (right; destruct H9; apply reachable_foot_valid in H6; apply H6).
+  assert (~ reachable g2 y_root x_root) by (intro; destruct H9; specialize (H16 _ H11); auto).
+  assert (vertices_at sh (vvalid (Graph_gen_redirect_parent g2 x_root y_root H6 H15 H11)) (Graph_gen_redirect_parent g2 x_root y_root H6 H15 H11) =
+          vertices_at sh (vvalid g2) (Graph_gen_redirect_parent g2 x_root y_root H6 H15 H11)). {
     apply vertices_at_Same_set. unfold Ensembles.Same_set, Ensembles.Included, Ensembles.In. simpl. intuition. }
 
   (* xRoot -> parent = yRoot; *)
@@ -317,13 +330,13 @@ Proof.
    (PROP  ()
     LOCAL (temp _xRoot (pointer_val_val x_root); temp _yRoot (pointer_val_val y_root))
     SEP   (data_at sh node_type (vgamma2cdata (vgamma g2 x_root)) (pointer_val_val x_root))).
-  rewrite H7. simpl vgamma2cdata.
+  rewrite H13. simpl vgamma2cdata.
   eapply semax_ram_seq';
     [ subst RamFrame RamFrame0; unfold abbreviate;
       repeat apply eexists_add_stats_cons; constructor
     | store_tac
     | abbreviate_semax_ram].
-  assert (force_val (sem_cast_neutral (pointer_val_val y_root)) = pointer_val_val y_root) by (destruct y_root; simpl; auto). rewrite H14. clear H14.
+  assert (force_val (sem_cast_neutral (pointer_val_val y_root)) = pointer_val_val y_root) by (destruct y_root; simpl; auto). rewrite H17. clear H17.
   change (@field_at CompSpecs sh node_type [] (Vint (Int.repr (Z.of_nat rankXRoot)), pointer_val_val y_root) (pointer_val_val x_root)) with
       (@data_at CompSpecs sh node_type (Vint (Int.repr (Z.of_nat rankXRoot)), pointer_val_val y_root) (pointer_val_val x_root)).
   unlocalize
@@ -331,26 +344,26 @@ Proof.
          LOCAL (temp _xRank (Vint (Int.repr (Z.of_nat rankXRoot))); temp _yRank (Vint (Int.repr (Z.of_nat rankYRoot)));
                 temp _xRoot (pointer_val_val x_root); temp _yRoot (pointer_val_val y_root);
                 temp _x (pointer_val_val x); temp _y (pointer_val_val y))
-    SEP (whole_graph sh (Graph_gen_redirect_parent g2 x_root y_root H10 H11 H12))).
+    SEP (whole_graph sh (Graph_gen_redirect_parent g2 x_root y_root H6 H15 H11))).
   Grab Existential Variables.
   Focus 2. {
-    simplify_ramif. rewrite H7. simpl vgamma2cdata. rewrite H13. apply (@graph_gen_redirect_parent_ramify _ (sSGG_VST sh)); auto. destruct H5.
-    apply reachable_foot_valid in H5. intro. subst y_root. apply (valid_not_null g2 null H5). simpl. auto.
+    simplify_ramif. rewrite H13. simpl vgamma2cdata. rewrite H16. apply (@graph_gen_redirect_parent_ramify _ (sSGG_VST sh)); auto. destruct H9.
+    apply reachable_foot_valid in H9. intro. subst y_root. apply (valid_not_null g2 null H9). simpl. auto.
   } Unfocus.
   Focus 1. {
-    unfold semax_ram. forward. apply (exp_right (Graph_gen_redirect_parent g2 x_root y_root H10 H11 H12)). entailer !.
-    apply (diff_root_union_1 g g1 g2 x y x_root y_root); auto.
+    unfold semax_ram. forward. apply (exp_right (Graph_gen_redirect_parent g2 x_root y_root H6 H15 H11)). entailer !. split.
+    - apply (diff_root_union_1 g g1 g2 x y x_root y_root); auto.
+    - rewrite H1 in *. rewrite H2 in *. rewrite <- Nat2Z.inj_lt in H5. destruct H9. apply uf_under_bound_redirect_parent_lt; auto.
   } Unfocus.
-
-  assert (weak_valid g2 x_root) by (right; destruct H4 as [? _]; rewrite <- H4; destruct H2; apply reachable_foot_valid in H2; apply H2).
-  assert (vvalid g2 y_root) by (destruct H5; apply reachable_foot_valid in H5; apply H5).
-  assert (~ reachable g2 x_root y_root) by (intro; rewrite (uf_equiv_root_the_same g1 g2) in H2; auto; destruct H2; specialize (H13 _ H12); auto).
-  assert (vertices_at sh (vvalid (Graph_gen_redirect_parent g2 y_root x_root H10 H11 H12)) (Graph_gen_redirect_parent g2 y_root x_root H10 H11 H12) =
-          vertices_at sh (vvalid g2) (Graph_gen_redirect_parent g2 y_root x_root H10 H11 H12)). {
+  assert (weak_valid g2 x_root) by (right; destruct H8; rewrite <- H6; destruct H4; apply reachable_foot_valid in H4; auto).
+  assert (vvalid g2 y_root) by (destruct H9; apply reachable_foot_valid in H9; apply H9).
+  assert (~ reachable g2 x_root y_root) by (intro; rewrite (uf_equiv_root_the_same g1 g2) in H4; auto; destruct H4; specialize (H17 _ H16); auto).
+  assert (vertices_at sh (vvalid (Graph_gen_redirect_parent g2 y_root x_root H6 H11 H16)) (Graph_gen_redirect_parent g2 y_root x_root H6 H11 H16) =
+          vertices_at sh (vvalid g2) (Graph_gen_redirect_parent g2 y_root x_root H6 H11 H16)). {
     apply vertices_at_Same_set. unfold Ensembles.Same_set, Ensembles.Included, Ensembles.In. simpl. intuition. }
   forward_if_tac
     (EX g': Graph,
-     PROP (uf_union g x y g')
+     PROP (uf_union g x y g' /\ uf_under_bound g')
           LOCAL (temp _xRank (Vint (Int.repr (Z.of_nat rankXRoot))); temp _yRank (Vint (Int.repr (Z.of_nat rankYRoot)));
                  temp _xRoot (pointer_val_val x_root); temp _yRoot (pointer_val_val y_root);
                  temp _x (pointer_val_val x); temp _y (pointer_val_val y))
@@ -363,13 +376,13 @@ Proof.
    (PROP  ()
     LOCAL (temp _xRoot (pointer_val_val x_root); temp _yRoot (pointer_val_val y_root))
     SEP   (data_at sh node_type (vgamma2cdata (vgamma g2 y_root)) (pointer_val_val y_root))).
-  rewrite H8. simpl vgamma2cdata.
+  rewrite H14. simpl vgamma2cdata.
   eapply semax_ram_seq';
     [ subst RamFrame RamFrame0; unfold abbreviate;
       repeat apply eexists_add_stats_cons; constructor
     | store_tac
     | abbreviate_semax_ram].
-  assert (force_val (sem_cast_neutral (pointer_val_val x_root)) = pointer_val_val x_root) by (destruct x_root; simpl; auto). rewrite H15. clear H15.
+  assert (force_val (sem_cast_neutral (pointer_val_val x_root)) = pointer_val_val x_root) by (destruct x_root; simpl; auto). rewrite H19. clear H19.
   change (@field_at CompSpecs sh node_type [] (Vint (Int.repr (Z.of_nat rankYRoot)), pointer_val_val x_root) (pointer_val_val y_root)) with
       (@data_at CompSpecs sh node_type (Vint (Int.repr (Z.of_nat rankYRoot)), pointer_val_val x_root) (pointer_val_val y_root)).
   unlocalize
@@ -377,15 +390,17 @@ Proof.
          LOCAL (temp _xRank (Vint (Int.repr (Z.of_nat rankXRoot))); temp _yRank (Vint (Int.repr (Z.of_nat rankYRoot)));
                 temp _xRoot (pointer_val_val x_root); temp _yRoot (pointer_val_val y_root);
                 temp _x (pointer_val_val x); temp _y (pointer_val_val y))
-    SEP (whole_graph sh (Graph_gen_redirect_parent g2 y_root x_root H10 H11 H12))).
+    SEP (whole_graph sh (Graph_gen_redirect_parent g2 y_root x_root H6 H11 H16))).
   Grab Existential Variables.
   Focus 2. {
-    simplify_ramif. rewrite H8. simpl vgamma2cdata. rewrite H13. apply (@graph_gen_redirect_parent_ramify _ (sSGG_VST sh)); auto. destruct H2.
-    apply reachable_foot_valid in H2. intro. subst x_root. apply (valid_not_null g1 null H2). simpl. auto.
+    simplify_ramif. rewrite H14. simpl vgamma2cdata. rewrite H17. apply (@graph_gen_redirect_parent_ramify _ (sSGG_VST sh)); auto. destruct H4.
+    apply reachable_foot_valid in H4. intro. subst x_root. apply (valid_not_null g1 null H4). simpl. auto.
   } Unfocus.
   Focus 1. {
-    unfold semax_ram. forward. apply (exp_right (Graph_gen_redirect_parent g2 y_root x_root H10 H11 H12)). entailer !.
-    apply (diff_root_union_2 g g1 g2 x y x_root y_root); auto.
+    unfold semax_ram. forward. apply (exp_right (Graph_gen_redirect_parent g2 y_root x_root H6 H11 H16)). entailer !. split.
+    - apply (diff_root_union_2 g g1 g2 x y x_root y_root); auto.
+    - rewrite H1 in *. rewrite H2 in *. rewrite <- Nat2Z.inj_lt in H18. apply uf_under_bound_redirect_parent_lt; auto.
+      rewrite (uf_equiv_root_the_same g1 g2) in H4; auto. destruct H4. auto.
   } Unfocus.
 
   (* yRoot -> parent = xRoot; *)
@@ -393,13 +408,13 @@ Proof.
    (PROP  ()
     LOCAL (temp _xRoot (pointer_val_val x_root); temp _yRoot (pointer_val_val y_root))
     SEP   (data_at sh node_type (vgamma2cdata (vgamma g2 y_root)) (pointer_val_val y_root))).
-  rewrite H8. simpl vgamma2cdata.
+  rewrite H14. simpl vgamma2cdata.
   eapply semax_ram_seq;
     [ subst RamFrame RamFrame0; unfold abbreviate;
       repeat apply eexists_add_stats_cons; constructor
     | store_tac
     | abbreviate_semax_ram].
-  assert (force_val (sem_cast_neutral (pointer_val_val x_root)) = pointer_val_val x_root) by (destruct x_root; simpl; auto). rewrite H15. clear H15.
+  assert (force_val (sem_cast_neutral (pointer_val_val x_root)) = pointer_val_val x_root) by (destruct x_root; simpl; auto). rewrite H19. clear H19.
   change (@field_at CompSpecs sh node_type [] (Vint (Int.repr (Z.of_nat rankYRoot)), pointer_val_val x_root) (pointer_val_val y_root)) with
       (@data_at CompSpecs sh node_type (Vint (Int.repr (Z.of_nat rankYRoot)), pointer_val_val x_root) (pointer_val_val y_root)).
   unlocalize
@@ -407,13 +422,13 @@ Proof.
          LOCAL (temp _xRank (Vint (Int.repr (Z.of_nat rankXRoot))); temp _yRank (Vint (Int.repr (Z.of_nat rankYRoot)));
                 temp _xRoot (pointer_val_val x_root); temp _yRoot (pointer_val_val y_root);
                 temp _x (pointer_val_val x); temp _y (pointer_val_val y))
-    SEP (whole_graph sh (Graph_gen_redirect_parent g2 y_root x_root H10 H11 H12))).
+    SEP (whole_graph sh (Graph_gen_redirect_parent g2 y_root x_root H6 H11 H16))).
   Grab Existential Variables.
   Focus 2. {
-    simplify_ramif. rewrite H8. simpl vgamma2cdata. rewrite H13. apply (@graph_gen_redirect_parent_ramify _ (sSGG_VST sh)); auto. destruct H2.
-    apply reachable_foot_valid in H2. intro. subst x_root. apply (valid_not_null g1 null H2). simpl. auto.
-  } Unfocus. clear H13.
-  remember (Graph_gen_redirect_parent g2 y_root x_root H10 H11 H12) as g3.
+    simplify_ramif. rewrite H14. simpl vgamma2cdata. rewrite H17. apply (@graph_gen_redirect_parent_ramify _ (sSGG_VST sh)); auto. destruct H4.
+    apply reachable_foot_valid in H4. intro. subst x_root. apply (valid_not_null g1 null H4). simpl. auto.
+  } Unfocus. clear H17.
+  remember (Graph_gen_redirect_parent g2 y_root x_root H6 H11 H16) as g3.
   assert (uf_union g x y g3) by (rewrite Heqg3; simpl; apply (diff_root_union_2 g g1 g2 x y x_root y_root); auto).
 
   (* xRoot -> rank = xRank + 1; *)
@@ -421,7 +436,7 @@ Proof.
    (PROP  ()
     LOCAL (temp _xRoot (pointer_val_val x_root); temp _xRank (Vint (Int.repr (Z.of_nat rankXRoot))))
     SEP   (data_at sh node_type (vgamma2cdata (vgamma g2 x_root)) (pointer_val_val x_root))).
-  rewrite H7. simpl vgamma2cdata.
+  rewrite H13. simpl vgamma2cdata.
   eapply semax_ram_seq';
     [ subst RamFrame RamFrame0; unfold abbreviate;
       repeat apply eexists_add_stats_cons; constructor
@@ -442,9 +457,11 @@ Proof.
     assert (vertices_at sh (vvalid (Graph_vgen g3 x_root (rankXRoot + 1)%nat)) (Graph_vgen g3 x_root (rankXRoot + 1)%nat) =
             vertices_at sh (vvalid g3) (Graph_vgen g3 x_root (rankXRoot + 1)%nat)). {
       apply vertices_at_Same_set. unfold Ensembles.Same_set, Ensembles.Included, Ensembles.In. simpl. intuition.
-    } rewrite H15. clear H15. rewrite H7. simpl vgamma2cdata. apply (@graph_vgen_ramify _ (sSGG_VST sh)).
-    - rewrite Heqg3. simpl. destruct H4 as [? _]; rewrite <- H4; destruct H2; apply reachable_foot_valid in H2; apply H2.
+    } rewrite H19. clear H19. rewrite H13. simpl vgamma2cdata. apply (@graph_vgen_ramify _ (sSGG_VST sh)).
+    - rewrite Heqg3. simpl. destruct H8 as [? _]. rewrite <- H8. destruct H4; apply reachable_foot_valid in H4; apply H4.
     - apply (graph_gen_redirect_parent_vgamma _ _ _ rankXRoot paXRoot) in Heqg3; auto.
   } Unfocus.
   unfold semax_ram. forward. apply (exp_right (Graph_vgen g3 x_root (rankXRoot + 1)%nat)). entailer !.
-Qed. (* 205.811 secs *)
+  rewrite H1 in *; rewrite H2 in *. assert (Z.of_nat (vlabel g2 x_root) = Z.of_nat (vlabel g2 y_root)) by (clear -H5 H18; intuition). apply Nat2Z.inj in H23.
+  simpl in H13. inversion H13. clear H26. apply uf_under_bound_redirect_parent_eq; auto. rewrite (uf_equiv_root_the_same g1 g2) in H4; auto. destruct H4. auto.
+Qed. (* 192.772 secs *)
